completed wf unit

WfActionT.v
@@ -1,293 +1,503 @@
 Require Export Bool Ascii String Fin List FunctionalExtensionality Psatz PeanoNat.
 Require Export Kami.Syntax.
 
-Print ActionT.
-Print Kind.
-Print fullType.
-Print unit.
-Print tt.
-Check tt.
+Inductive Failure :=
+  | NativeReg : string -> Failure
+  | NativeLetExpr : Failure
+  | NativeReadNondet : Failure
+  | RegNotFound : string -> Failure
+  | HideMethodNotFound : string -> Failure
+  | RegKindMismatch : string -> FullKind -> FullKind -> Failure
+  | DuplicateMethod : string -> Signature -> Signature -> Failure
+  | DuplicateRegister : string -> FullKind -> FullKind -> Failure
+  | DuplicateRule : string -> Failure.
 
-Fixpoint WfActionT_unit {k} (regs : list (string * {x : FullKind & RegInitValT x})) (a : ActionT (fun _ => unit) k) : bool :=
-                             match a with
-                             | MCall meth s e cont => WfActionT_unit regs (cont tt)
-                             | LetExpr k' e cont => match k' return (fullType (fun _ => unit) k' -> ActionT (fun _ => unit) k) -> bool with
-                                                   | SyntaxKind k'' => fun cont => WfActionT_unit regs (cont tt)
-                                                   | @NativeKind k'' v => fun cont => false
-                                                   end cont
-                             | LetAction k a cont => WfActionT_unit regs a && WfActionT_unit regs (cont tt)
-                             | ReadNondet k' cont => match k' return (fullType (fun _ => unit) k' -> ActionT (fun _ => unit) k) -> bool with
-                                                    | SyntaxKind k'' => fun cont => WfActionT_unit regs (cont tt)
-                                                    | @NativeKind k'' v => fun cont => false
-                                                    end cont
-                             | ReadReg r k' cont => match lookup String.eqb r regs with
-                                                    | None => false
-                                                    | Some (existT k'' _) =>
-                                                      match k' return (fullType (fun _ => unit) k' -> ActionT (fun _ => unit) k) -> bool with
-                                                      | SyntaxKind k''' => match k'' with
-                                                                           | SyntaxKind k'''' => fun cont => Kind_decb k''' k'''' && WfActionT_unit regs (cont tt)
-                                                                           | @NativeKind k'''' v => fun cont => false
-                                                                           end
-                                                      | @NativeKind k''' v => fun cont => false
-                                                      end cont
-                                                   end
-                             | WriteReg r k' e cont => match lookup String.eqb r regs with
-                                                     | None => false
-                                                     | Some (existT k'' _) =>
-                                                        match k',k'' with
-                                                        | SyntaxKind k''',SyntaxKind k'''' => Kind_decb k''' k'''' && WfActionT_unit regs cont
-                                                        | _,_ => false
-                                                        end
-                                                     end
-                             | IfElse cond k' atrue afalse cont => (WfActionT_unit regs atrue) && (WfActionT_unit regs afalse) && (WfActionT_unit regs (cont tt))
-                             | Sys l cont => WfActionT_unit regs cont
-                             | Return e => true
-                             (*| _ => false*)
-                             end.
+Fixpoint WfActionT_unit {k} (regs : list (string * {x : FullKind & RegInitValT x})) (a : ActionT (fun _ => unit) k) : list Failure :=
+  match a with
+  | MCall meth s e cont => WfActionT_unit regs (cont tt)
+  | LetExpr (SyntaxKind k'') e cont => WfActionT_unit regs (cont tt)
+  | LetExpr (NativeKind t c) e cont => NativeLetExpr :: WfActionT_unit regs (cont c)
+  | LetAction k a cont => WfActionT_unit regs a ++ WfActionT_unit regs (cont tt)
+  | ReadNondet (SyntaxKind k') cont => WfActionT_unit regs (cont tt)
+  | ReadNondet (NativeKind t c) cont => NativeReadNondet :: WfActionT_unit regs (cont c)
+  | ReadReg r (SyntaxKind k') cont => 
+      match lookup String.eqb r regs with
+      | Some (existT (SyntaxKind k'') _) => (if Kind_decb k' k'' then [] else [RegKindMismatch r (SyntaxKind k') (SyntaxKind k'')]) ++ WfActionT_unit regs (cont tt)
+      | Some (existT (NativeKind t c) _) => [RegKindMismatch r (SyntaxKind k') (NativeKind c)]
+      | None => [RegNotFound r]
+      end
+  | ReadReg r (NativeKind t c) cont => [NativeReg r]
+  | WriteReg r (SyntaxKind k') e cont =>
+      match lookup String.eqb r regs with
+      | Some (existT (SyntaxKind k'') _) => if Kind_decb k' k'' then WfActionT_unit regs cont else RegKindMismatch r (SyntaxKind k') (SyntaxKind k'') :: WfActionT_unit regs cont
+      | Some (existT (NativeKind t c) _) => [RegKindMismatch r (SyntaxKind k') (NativeKind c)]
+      | None => [RegNotFound r]
+      end
+  | WriteReg r (NativeKind t c) e cont => NativeReg r :: WfActionT_unit regs cont
+  | IfElse cond k' atrue afalse cont => WfActionT_unit regs atrue ++ WfActionT_unit regs afalse ++ WfActionT_unit regs (cont tt)
+  | Sys l cont => WfActionT_unit regs cont
+  | Return e => []
+  end.
 
-Fixpoint has_native {k} (a : ActionT (fun _ => unit) k) : bool :=
-                         match a with
-                         | MCall meth s e cont => has_native (cont tt)
-                         | LetExpr k' e cont => match k' return (fullType (fun _ => unit) k' -> ActionT (fun _ => unit) k) -> bool with
-                                                | SyntaxKind k'' => fun cont => has_native (cont tt)
-                                                | @NativeKind k'' v => fun cont => true
-                                                end cont
-                         | LetAction k a cont => has_native a || has_native (cont tt)
-                         | ReadNondet k' cont => match k' return (fullType (fun _ => unit) k' -> ActionT (fun _ => unit) k) -> bool with
-                                                 | SyntaxKind k'' => fun cont => has_native (cont tt)
-                                                 | @NativeKind k'' v => fun cont => true
-                                                 end cont
-                         | ReadReg r k' cont => match k' return (fullType (fun _ => unit) k' -> ActionT (fun _ => unit) k) -> bool with
-                                                | SyntaxKind k''' => fun cont => has_native (cont tt)
-                                                | @NativeKind k''' v => fun cont => true
-                                                end cont
-                         | WriteReg r k' e cont => match k' with
-                                                   | SyntaxKind k'' => has_native cont
-                                                   | _ => true
-                                                   end
-                         | IfElse cond k' atrue afalse cont => (has_native atrue) || (has_native afalse) || (has_native (cont tt))
-                         | Sys l cont => has_native cont
-                         | Return e => false
-                         (*| _ => false*)
-                         end.
-                        
+Definition WfBaseModule_rules_unit(m : BaseModule) :=
+  List.fold_right (fun rule fs => WfActionT_unit (getRegisters m) rule ++ fs) [] (map (fun r => snd r _) (getRules m)).
 
-Theorem test: forall regs k (a:ActionT (fun _ => unit) k), (WfActionT_unit regs a && negb(has_native a))=true -> @WfActionT_new regs (fun _ => unit) k a.
+Definition action_from_MethodT : (string * {x : Signature & MethodT x}) -> {k : _ & ActionT (fun _ => unit) k}.
 Proof.
   intros.
-  induction a.
-  - simpl.
-    intros.
-    eapply H0.
-    simpl in H.
-    simpl.
-    destruct x.
-    apply H.
-  - simpl.
-    intros.
-    destruct k.
-    + eapply H0.
-      simpl in x.
-      destruct x.
-      simpl in H.
-      apply H.
-    + simpl.
-      simpl in H.
-      inversion H.
-  - simpl.
-    intros.
-    split.
-    + apply IHa.
-      remember (WfActionT_unit regs a).
-      destruct b.
-      * remember (has_native a).
-        destruct b.
-        -- simpl in H.
-           rewrite <- Heqb0 in H.
-           simpl in H.
-           rewrite andb_false_r in H.
-           inversion H.
-        -- reflexivity.
-      * simpl in H.
-        rewrite <- Heqb in H.
-        rewrite andb_false_l in H.
-        inversion H.
-    + intros.
-      eapply H0.
-      destruct x.
-      simpl in H.
-      remember (WfActionT_unit regs (a0 tt)).
-      destruct b.
-      * remember (has_native (a0 tt)).
-        destruct b.
-        -- simpl in H.
-           rewrite orb_true_r in H.
-           simpl in H.
-           rewrite andb_false_r in H.
-           inversion H.
-        -- reflexivity.
-      * simpl in H.
-        rewrite andb_false_r in H.
-        rewrite andb_false_l in H.
-        inversion H.
-  - simpl.
-    intros.
-    destruct k.
-    + eapply H0.
-      simpl in x.
-      destruct x.
-      simpl in H.
-      apply H.
-    + simpl.
-      simpl in H.
-      inversion H.
-  - simpl.
-    intros.
-    destruct k.
-    + remember (lookup String.eqb r regs).
-      destruct o.
-      * destruct s.
-        split.
-        -- destruct x.
-           ++ simpl in H.
-              rewrite <- Heqo in H.
-              remember (Kind_decb k k0).
-              destruct b.
-              ** symmetry in Heqb.
-                 rewrite Kind_decb_eq in Heqb.
-                 subst.
-                 reflexivity.
-              ** rewrite andb_false_l in H.
-                 inversion H.
-           ++ simpl in H.
-              rewrite <- Heqo in H.
-              rewrite andb_false_l in H.
-              inversion H.
-        -- simpl in H.
-           rewrite <- Heqo in H.
-           destruct x.
-           ++ remember (Kind_decb k k0).
-              destruct b.
-              ** symmetry in Heqb.
-                 rewrite Kind_decb_eq in Heqb.
-                 subst.
-                 simpl.
-                 intros.
-                 apply H0.
-                 destruct x.
-                 rewrite andb_true_l in H.
-                 apply H.
-              ** rewrite andb_false_l in H.
-                 inversion H.
-           ++ rewrite andb_false_l in H.
-              inversion H.
-      * simpl in H.
-        rewrite <- Heqo in H.
-        rewrite andb_false_l in H.
-        inversion H.
-    + simpl in H.
-      rewrite andb_false_r in H.
-      inversion H.
-  - simpl.
-    remember (lookup String.eqb r regs).
-    destruct o.
-    + destruct s.
-      split.
-      * destruct x.
-        ++ simpl in H.
-           rewrite <- Heqo in H.
-           destruct k.
-           -- remember (Kind_decb k k0).
-              destruct b.
-              ** symmetry in Heqb.
-                 rewrite Kind_decb_eq in Heqb.
-                 subst.
-                 reflexivity.
-              ** rewrite andb_false_l in H.
-                 inversion H.
-           -- rewrite andb_false_l in H.
-              inversion H.
-        ++ simpl in H.
-           rewrite <- Heqo in H.
-           destruct k.
-           -- rewrite andb_false_l in H.
-              inversion H.
-           -- rewrite andb_false_l in H.
-              inversion H.
-      * simpl in H.
-        rewrite <- Heqo in H.
-        destruct k.
-        ++ destruct x.
-           -- apply IHa.
-              simpl.
-              remember (Kind_decb k k0).
-              destruct b.
-              ** rewrite andb_true_l in H.
-                 apply H.
-              ** rewrite andb_false_l in H.
-                 inversion H.
-           -- rewrite andb_false_l in H.
-              inversion H.
-        ++ rewrite andb_false_l in H.
-           inversion H.
-    + simpl in H.
-      rewrite <- Heqo in H.
-      rewrite andb_false_l in H.
-      inversion H.
-  - simpl in H.
-    simpl.
-    split.
-    + apply IHa1.
-      remember (WfActionT_unit regs a1).
-      destruct b.
-      * remember (has_native a1).
-        destruct b.
-        ++ rewrite orb_true_l in H.
-           simpl in H.
-           rewrite andb_false_r in H.
-           inversion H.
-        ++ reflexivity.
-      * rewrite andb_false_l in H.
-        inversion H.
-    + split.
-      * apply IHa2.
-        remember (WfActionT_unit regs a2).
-        destruct b.
-        ++ remember (has_native a2).
-           destruct b.
-           -- rewrite orb_true_r in H.
-              rewrite orb_true_l in H.
-              simpl in H.
-              rewrite andb_false_r in H.
-              inversion H.
-           -- reflexivity.
-        ++ rewrite andb_false_r in H.
-           rewrite andb_false_l in H.
-           inversion H.
-      * intros.
-        destruct x.
-        apply H0.
-        remember (WfActionT_unit regs (a3 tt)).
-        destruct b.
-        ++ remember (has_native (a3 tt)).
-           destruct b.
-           -- rewrite orb_true_r in H.
-              simpl in H.
-              rewrite andb_false_r in H.
-              inversion H.
-           -- reflexivity.
-        ++ rewrite andb_false_r in H.
-           rewrite andb_false_l in H.
-           inversion H.
-  - simpl.
-    apply IHa.
-    simpl in H.
-    apply H.
-  - simpl.
-    apply I.
+  destruct X.
+  destruct s0.
+  unfold MethodT in m.
+  pose (m (fun _ => unit)).
+  exists (snd x).
+  exact (a tt).
+Defined.
+
+Definition WfBaseModule_methods_unit(m : BaseModule) :=
+  List.fold_right (fun meth fs => WfActionT_unit (getRegisters m) (projT2 (action_from_MethodT meth)) ++ fs) [] (getMethods m).
+
+Fixpoint find_dups_aux{X}(acc ps : list (string * X)) : list (string * X * X) :=
+  match ps with
+  | [] => []
+  | p::qs => match lookup String.eqb (fst p) acc with
+             | Some x => (fst p, snd p, x) :: find_dups_aux acc qs
+             | None => find_dups_aux (p::acc) qs
+             end
+  end.
+
+Definition find_dups{X} : list (string * X) -> list (string * X * X) := find_dups_aux [].
+
+Definition test := [("a", 5); ("b", 156); ("c", 3); ("a", 4); ("d", 46); ("b", 75)].
+
+Definition WfBaseModule_unit(m : BaseModule) :=
+     map (fun '(s,x1,x2) => DuplicateMethod s (projT1 x1) (projT1 x2)) (find_dups (getMethods m))
+  ++ map (fun '(s,x1,x2) => DuplicateRegister s (projT1 x1) (projT1 x2)) (find_dups (getRegisters m))
+  ++ map (fun '(s,x1,x2) => DuplicateRule s) (find_dups (getRules m))
+  ++ WfBaseModule_rules_unit m
+  ++ WfBaseModule_methods_unit m.
+
+Fixpoint find_overlaps{X}(ps qs : list (string * X)) : list (string * X * X) :=
+  match ps with
+  | [] => []
+  | p::ps' => match lookup String.eqb (fst p) qs with
+              | Some x => (fst p,snd p,x) :: find_overlaps ps' qs
+              | None => find_overlaps ps' qs
+              end
+  end.
+
+Fixpoint WfConcatActionT_unit{k}(a : ActionT (fun _ => unit) k)(m : Mod) : list Failure :=
+  match a with
+  | MCall meth s e cont => (if existsb (String.eqb meth) (getHidden m) then [HideMethodNotFound meth] else [])  ++ WfConcatActionT_unit (cont tt) m
+  | LetExpr (SyntaxKind k') e cont => WfConcatActionT_unit (cont tt) m
+  | LetExpr (NativeKind t c) e cont => NativeLetExpr :: WfConcatActionT_unit (cont c) m
+  | LetAction k a cont => WfConcatActionT_unit a m ++ WfConcatActionT_unit (cont tt) m
+  | ReadNondet (SyntaxKind k') cont => WfConcatActionT_unit (cont tt) m
+  | ReadNondet (NativeKind t c) cont => NativeReadNondet :: WfConcatActionT_unit (cont c) m
+  | ReadReg r (SyntaxKind k') cont => WfConcatActionT_unit (cont tt) m
+  | ReadReg r (NativeKind t c) cont => NativeReg r :: WfConcatActionT_unit (cont c) m
+  | WriteReg r k e a => WfConcatActionT_unit a m
+  | IfElse e k a1 a2 cont => WfConcatActionT_unit a1 m ++ WfConcatActionT_unit a2 m ++ WfConcatActionT_unit (cont tt) m
+  | Sys _ a => WfConcatActionT_unit a m
+  | Return _ => []
+  end.
+
+Definition WfConcat_unit m1 m2 :=
+     List.fold_right (fun rule fs => WfConcatActionT_unit rule m2 ++ fs) [] (map (fun r => snd r _) (getAllRules m1))
+  ++ List.fold_right (fun meth fs => WfConcatActionT_unit (projT2 meth) m2 ++ fs) [] (map action_from_MethodT (getAllMethods m1)).
+
+Fixpoint WfMod_unit(m : Mod) :=
+  match m with
+  | Base m => WfBaseModule_unit m
+  | HideMeth m s => match lookup String.eqb s (getAllMethods m) with
+                    | Some _ => WfMod_unit m
+                    | None => HideMethodNotFound s :: WfMod_unit m
+                    end
+  | ConcatMod m1 m2 =>
+         WfMod_unit m1
+      ++ WfMod_unit m2
+      ++ map (fun '(s,x1,x2) => DuplicateRegister s (projT1 x1) (projT1 x2)) (find_overlaps (getAllRegisters m1) (getAllRegisters m2))
+      ++ map (fun '(s,x1,x2) => DuplicateRule s) (find_overlaps (getAllRules m1) (getAllRules m2))
+      ++ map (fun '(s,x1,x2) => DuplicateMethod s (projT1 x1) (projT1 x2)) (find_overlaps (getAllMethods m1) (getAllMethods m2))
+      ++ WfConcat_unit m1 m2
+      ++ WfConcat_unit m2 m1
+  end.
+
+Section Proofs.
+
+Lemma In_map_fst : forall {X Y}(x : X) ps, In x (map fst ps) -> exists y : Y, In (x,y) ps.
+Proof.
+  induction ps; intros.
+  - destruct H.
+  - destruct H.
+    exists (snd a).
+    left.
+    destruct a.
+    simpl in *; congruence.
+    destruct (IHps H) as [y Hy].
+    exists y.
+    right; exact Hy.
 Qed.
 
-Axiom test2: forall regs k (a:forall ty k, ActionT ty k), @WfActionT_new regs (fun _ => unit) k (a (fun _ => unit) k) ->
-                                                          forall ty k, @WfActionT_new regs ty k (a ty k).
+Lemma In_lookup : forall {X} str (ps : list (string * X)), In str (map fst ps) -> exists x, lookup String.eqb str ps = Some x.
+Proof.
+  induction ps; intros.
+  - destruct H.
+  - destruct H.
+    + exists (snd a).
+      unfold lookup.
+      simpl.
+      rewrite H.
+      rewrite String.eqb_refl.
+      reflexivity.
+    + destruct a.
+      rewrite lookup_cons.
+      destruct String.eqb eqn:G.
+      * exists x; auto.
+      * auto.
+Qed.
+
+Lemma lookup_In : forall {X} str (ps : list (string * X)) x, lookup String.eqb str ps = Some x -> In str (map fst ps).
+Proof.
+  induction ps.
+  - intros; discriminate.
+  - intros.
+    destruct a.
+    rewrite lookup_cons in H.
+    destruct String.eqb eqn:G.
+    + left.
+      rewrite String.eqb_eq in G; simpl; congruence.
+    + right.
+      apply (IHps x); auto.
+Qed.
+
+Lemma find_dups_aux_NoDup : forall {X}(ps acc : list (string * X)), find_dups_aux acc ps = [] -> NoDup (map fst ps) /\ forall str, In str (map fst ps) -> ~ In str (map fst acc).
+Proof.
+  induction ps; intros.
+  - split.
+    + constructor.
+    + intros.
+      destruct H0.
+  - split.
+    + simpl in H.
+      destruct lookup eqn:G in H.
+      * discriminate.
+      * destruct (IHps _ H).
+        constructor.
+        ** intro.
+           apply (H1 (fst a)).
+           exact H2.
+           left; auto.
+        ** exact H0.
+    + simpl in H.
+      destruct lookup eqn:G in H.
+      * discriminate.
+      * intros.
+        destruct (IHps _ H).
+        intro.
+        destruct H0.
+        ** destruct (In_lookup str acc H3) as [x Hx].
+           rewrite H0 in G.
+           rewrite Hx in G.
+           discriminate.
+        ** apply (H2 str); auto.
+           right; auto.
+Qed.
+
+Lemma find_dups_NoDups : forall {X}(ps : list (string * X)), find_dups ps = [] -> NoDup (map fst ps).
+Proof.
+  intros.
+  eapply find_dups_aux_NoDup.
+  exact H.
+Qed.
+
+Lemma WfActionT_unit_correct : forall lret m (a : ActionT _ lret), WfActionT_unit (getRegisters m) a = [] -> WfActionT_new (getRegisters m) a.
+Proof.
+  induction a; simpl; intros.
+  - apply H; destruct x; auto.
+  - apply H.
+    destruct k.
+    + destruct x; auto.
+    + discriminate H0.
+  - split.
+    + apply IHa.
+      destruct (app_eq_nil _ _ H0); auto.
+    + intro; apply H.
+      destruct (app_eq_nil _ _ H0); destruct x; auto.
+  - apply H.
+    destruct k.
+    + destruct x; auto.
+    + discriminate.
+  - destruct k.
+    + destruct lookup eqn:G.
+      * destruct s.
+        destruct x.
+        ** destruct Kind_decb eqn:G0.
+           *** split.
+               **** rewrite Kind_decb_eq in G0; congruence.
+               **** intros []; apply H; auto.
+           *** discriminate.
+        ** discriminate.
+      * discriminate.
+    + discriminate.
+  - destruct k.
+    + destruct lookup eqn:G.
+      * destruct s.
+        destruct x.
+        ** destruct Kind_decb eqn:G0.
+           *** split.
+               **** rewrite Kind_decb_eq in G0; congruence.
+               **** auto.
+           *** discriminate.
+        ** discriminate.
+      * discriminate.
+    + discriminate.
+  - destruct (app_eq_nil _ _ H0); clear H0.
+    destruct (app_eq_nil _ _ H2); clear H2.
+    repeat split; auto.
+    intros []; auto.
+  - auto.
+  - exact I.
+Qed.
+
+Lemma fold_right_empty_lemma : forall {X Y}(f : X -> list Y)(xs : list X),
+  fold_right (fun x ys => f x ++ ys) [] xs = [] -> forall x, In x xs -> f x = [].
+Proof.
+  induction xs; intros.
+  - destruct H0.
+  - simpl in H.
+    destruct (app_eq_nil _ _ H).
+    destruct H0.
+    + congruence.
+    + auto.
+Qed.
+
+Lemma WfBaseModule_rules_unit_In : forall m, WfBaseModule_rules_unit m = [] -> forall rule, In rule (getRules m) -> WfActionT_unit (getRegisters m) (snd rule _) = [].
+Proof.
+  intros.
+  apply (fold_right_empty_lemma _ _ H).
+  apply (@in_map _ _ (fun r : string * (forall x : Kind -> Type, ActionT x Void) => snd r (fun _ => unit))); auto.
+Qed.
+
+Lemma WfBaseModule_rules_unit_correct : forall m, WfBaseModule_rules_unit m = [] -> forall rule, In rule (getRules m) ->
+  WfActionT_new (getRegisters m) (snd rule (fun _ => unit)).
+Proof.
+  intros.
+  apply WfActionT_unit_correct.
+  apply WfBaseModule_rules_unit_In; auto.
+Qed.
+
+Lemma In_WfRules : forall ty regs rules, (forall rule, In rule rules -> WfActionT_new regs (snd rule ty)) -> WfRules ty regs rules.
+Proof.
+  induction rules; intros; simpl.
+  - exact I.
+  - split.
+    + apply H.
+      left; auto.
+    + apply IHrules.
+      intros.
+      apply H.
+      right; auto.
+Qed.
+
+Lemma WfBaseModule_methods_unit_In : forall m, WfBaseModule_methods_unit m = [] -> forall meth, In meth (getMethods m) -> WfActionT_unit (getRegisters m) (projT2 (snd meth) _ tt) = [].
+Proof.
+  intros.
+  unfold WfBaseModule_methods_unit in H.
+  pose @fold_right_empty_lemma.
+  pose (@fold_right_empty_lemma _ _ _ _ H).
+  unfold action_from_MethodT in e0.
+  pose (e0 meth).
+  destruct meth.
+  destruct s0.
+  simpl in e1.
+  apply e1.
+  exact H0.
+Qed.
+
+Lemma WfBaseModule_methods_unit_correct : forall m, WfBaseModule_methods_unit m = [] -> forall meth, In meth (getMethods m) ->
+  WfActionT_new (getRegisters m) (projT2 (snd meth) (fun _ => unit) tt).
+Proof.
+  intros.
+  apply WfActionT_unit_correct.
+  apply WfBaseModule_methods_unit_In; auto.
+Qed.
 
 
+Lemma In_WfMethods : forall ty regs meths, (forall (meth : string * {x : Signature & MethodT x}) v, In meth meths -> @WfActionT_new ty regs _ (projT2 (snd meth) _ v)) -> WfMeths ty regs meths.
+Proof.
+  induction meths; intros; simpl.
+  - exact I.
+  - split.
+    + intro; apply H.
+      left; auto.
+    + apply IHmeths.
+      intros.
+      apply H.
+      right; auto.
+Qed.
+
+Lemma WfBaseModule_unit_correct : forall m, WfBaseModule_unit m = [] -> WfBaseModule_new (fun _ => unit) m.
+Proof.
+  unfold WfBaseModule_unit, WfBaseModule_new.
+  intros.
+  destruct (app_eq_nil _ _ H); clear H.
+  destruct (app_eq_nil _ _ H1); clear H1.
+  destruct (app_eq_nil _ _ H2); clear H2.
+  destruct (app_eq_nil _ _ H3); clear H3.
+  repeat split.
+  - apply In_WfRules.
+    intros.
+    apply WfBaseModule_rules_unit_correct; auto.
+  - apply In_WfMethods.
+    intros meth [].
+    apply WfBaseModule_methods_unit_correct; auto.
+  - apply find_dups_NoDups.
+    eapply map_eq_nil.
+    exact H0.
+  - apply find_dups_NoDups.
+    eapply map_eq_nil.
+    exact H.
+  - apply find_dups_NoDups.
+    eapply map_eq_nil.
+    exact H1.
+Qed.
+
+Lemma find_overlaps_DisjKey : forall {X}(ps qs : list (string * X)), find_overlaps ps qs = [] -> DisjKey ps qs.
+Proof.
+  induction ps; intros qs Hoverlaps str.
+  - left; simpl; auto.
+  - simpl in Hoverlaps.
+    destruct lookup eqn:G.
+    + discriminate.
+    + destruct (IHps qs Hoverlaps str).
+      * destruct (fst a =? str) eqn:G0.
+        ** right.
+           intro.
+           destruct (In_lookup _ _ H0).
+           rewrite String.eqb_eq in G0.
+            rewrite G0 in G.
+            rewrite H1 in G.
+            discriminate.
+        ** left.
+           intros [|].
+           *** rewrite H0 in G0.
+               rewrite String.eqb_refl in G0.
+               discriminate.
+           *** auto.
+      * tauto.
+Qed.
+
+Lemma WfConcatActionT_unit_correct : forall {lret} m (a : ActionT (fun _ => unit) lret),
+  WfConcatActionT_unit a m = [] -> WfConcatActionT_new a m.
+Proof.
+  induction a; simpl; intros.
+  - split.
+    + destruct existsb eqn:G.
+      * discriminate.
+      * Search existsb In.
+        intro.
+        assert (existsb (String.eqb meth) (getHidden m) = true).
+        ** apply existsb_exists.
+           exists meth; split.
+           *** auto.
+           *** apply String.eqb_refl.
+        ** rewrite H2 in G; discriminate.
+    + destruct x.
+      apply H.
+      destruct (app_eq_nil _ _ H0); auto.
+  - destruct k.
+    + destruct x; auto.
+    + discriminate.
+  - destruct (app_eq_nil _ _ H0); clear H0.
+    split.
+    + auto.
+    + destruct x; auto.
+  - destruct k.
+    + destruct x; auto.
+    + discriminate.
+  - destruct k.
+    + destruct x; auto.
+    + discriminate.
+  - auto.
+  - destruct (app_eq_nil _ _ H0); clear H0.
+    destruct (app_eq_nil _ _ H2); clear H2.
+    repeat split.
+    + auto.
+    + auto.
+    + destruct x; auto.
+  - auto.
+  - exact I.
+Qed.
+
+Lemma in_map2 : forall (A B : Type)(f : A -> B)(l : list A)(x : A)(y : B), y = f x -> In x l -> In y (map f l).
+Proof.
+  intros.
+  rewrite H.
+  apply in_map; auto.
+Qed.
+
+Theorem WfMod_unit_correct : forall m, WfMod_unit m = [] -> WfMod_new (fun _ => unit) m.
+Proof.
+  induction m; simpl; intro.
+  - apply WfBaseModule_unit_correct; auto.
+  - destruct lookup eqn:G in H.
+    + split.
+      * eapply lookup_In.
+        exact G.
+      * auto.
+    + discriminate.
+  - destruct (app_eq_nil _ _ H); clear H.
+    destruct (app_eq_nil _ _ H1); clear H1.
+    destruct (app_eq_nil _ _ H2); clear H2.
+    destruct (app_eq_nil _ _ H3); clear H3.
+    destruct (app_eq_nil _ _ H4); clear H4.
+    destruct (app_eq_nil _ _ H5); clear H5.
+    destruct (app_eq_nil _ _ H4); clear H4.
+    destruct (app_eq_nil _ _ H6); clear H6.
+    repeat split.
+    + apply find_overlaps_DisjKey.
+      eapply map_eq_nil.
+      exact H1.
+    + apply find_overlaps_DisjKey.
+      eapply map_eq_nil.
+      exact H2.
+    + apply find_overlaps_DisjKey.
+      eapply map_eq_nil.
+      exact H3.
+    + auto.
+    + auto.
+    + intros; apply WfConcatActionT_unit_correct.
+      apply (@fold_right_empty_lemma _ _ _ _ H5).
+      apply (@in_map _ _ (fun r : string * (forall x : Kind -> Type, ActionT x Void) => snd r (fun _ => unit))); auto.
+    + intros; apply WfConcatActionT_unit_correct.
+      unfold action_from_MethodT in H7.
+      destruct v.
+      pose (@fold_right_empty_lemma _ _ _ _ H7).
+      pose (e (action_from_MethodT meth)).
+      destruct meth.
+      destruct s0.
+      simpl.
+      unfold action_from_MethodT in e0.
+      simpl in e0.
+      apply e0.
+      apply (@in_map2 _ _ _ _ ((s, existT MethodT x m))).
+      reflexivity.
+      exact H6.
+    + intros; apply WfConcatActionT_unit_correct.
+      apply (@fold_right_empty_lemma _ _ _ _ H4).
+      apply (@in_map _ _ (fun r : string * (forall x : Kind -> Type, ActionT x Void) => snd r (fun _ => unit))); auto.
+    + intros; apply WfConcatActionT_unit_correct.
+      unfold action_from_MethodT in H8.
+      destruct v.
+      pose (@fold_right_empty_lemma _ _ _ _ H8).
+      pose (e (action_from_MethodT meth)).
+      destruct meth.
+      destruct s0.
+      simpl.
+      unfold action_from_MethodT in e0.
+      simpl in e0.
+      apply e0.
+      apply (@in_map2 _ _ _ _ ((s, existT MethodT x m))).
+      reflexivity.
+      exact H6.
+Qed.
